policies/NullPolicy.v
@@ -31,56 +31,54 @@ Module NullPolicy <: Policy.
   Definition DefLT   : loc_tag := tt.
   Definition InitT   : val_tag := tt.
   
-  Definition print_tag (t:tag) : string := "tt".
+  Definition print_vt (t:val_tag) : string := "tt".
+  Definition print_ct (t:control_tag) : string := "tt".
+  Definition print_lt (t:loc_tag) : string := "tt".
+
+  Definition policy_state : Type := unit.
+  Definition log (pstate: policy_state) (msg: string) : policy_state := tt.
+  Definition dump (pstate: policy_state) : string := "".
   
-  (* anaaktge does not inherit, more like impersonates *)
-  Inductive PolicyResult (A: Type) :=
-  | PolicySuccess (res: A)
-  | PolicyFail (r: string) (params: list tag).
-
-  Arguments PolicySuccess {_} _. 
-  Arguments PolicyFail {_} _ _.
-
   Definition CallT (l:loc) (pct: control_tag) (pt: val_tag) : PolicyResult control_tag :=
-    PolicySuccess tt.
+    Success tt.
 
   Definition ArgT (l:loc) (pct: control_tag) (fpt vt: val_tag) (idx:nat) (ty: type) :
-    PolicyResult (control_tag * val_tag) := PolicySuccess (tt,tt).
+    PolicyResult (control_tag * val_tag) := Success (tt,tt).
 
   Definition RetT (l:loc) (pct_clr pct_cle: control_tag) (vt : val_tag) :
-    PolicyResult (control_tag * val_tag) := PolicySuccess (tt,tt).
+    PolicyResult (control_tag * val_tag) := Success (tt,tt).
 
   Definition LoadT (l:loc) (pct: control_tag) (pt vt: val_tag) (lts: list loc_tag) :
-    PolicyResult val_tag := PolicySuccess tt.
+    PolicyResult val_tag := Success tt.
 
   Definition StoreT (l:loc) (pct: control_tag) (pt vt: val_tag) (lts: list loc_tag) :
-    PolicyResult (control_tag * val_tag * list loc_tag) := PolicySuccess (tt, tt, [tt]).
+    PolicyResult (control_tag * val_tag * list loc_tag) := Success (tt, tt, [tt]).
 
   Definition AccessT (l:loc) (pct: control_tag) (vt: val_tag) :
-    PolicyResult val_tag := PolicySuccess tt.
+    PolicyResult val_tag := Success tt.
 
   Definition AssignT (l:loc) (pct: control_tag) (vt1 vt2: val_tag) :
-    PolicyResult (control_tag * val_tag) := PolicySuccess (tt,tt).
+    PolicyResult (control_tag * val_tag) := Success (tt,tt).
 
   Definition UnopT (l:loc) (op : unary_operation) (pct: control_tag) (vt: val_tag) :
-    PolicyResult (control_tag * val_tag) := PolicySuccess (tt, tt).
+    PolicyResult (control_tag * val_tag) := Success (tt, tt).
 
   Definition BinopT (l:loc) (op : binary_operation) (pct: control_tag) (vt1 vt2: val_tag) :
-    PolicyResult (control_tag * val_tag) := PolicySuccess (tt, tt).
+    PolicyResult (control_tag * val_tag) := Success (tt, tt).
 
-  Definition ConstT (l:loc) (pct: control_tag) : PolicyResult val_tag := PolicySuccess tt.
+  Definition ConstT (l:loc) (pct: control_tag) : PolicyResult val_tag := Success tt.
 
   Definition SplitT (l:loc) (pct: control_tag) (vt: val_tag) (id : option ident) :
-    PolicyResult control_tag := PolicySuccess tt.
+    PolicyResult control_tag := Success tt.
 
   Definition LabelT (l:loc) (pct: control_tag) (id : ident) : PolicyResult control_tag :=
-    PolicySuccess tt.
+    Success tt.
 
   Definition ExprSplitT (l:loc) (pct: control_tag) (vt : val_tag) : PolicyResult control_tag :=
-    PolicySuccess tt.
+    Success tt.
 
   Definition ExprJoinT (l:loc) (pct: control_tag) (vt: val_tag) :
-    PolicyResult (control_tag * val_tag) := PolicySuccess (tt,tt).
+    PolicyResult (control_tag * val_tag) := Success (tt,tt).
 
   Definition GlobalT (ce : composite_env) (id : ident) (ty : type) : val_tag * val_tag * loc_tag :=
     (tt, tt, tt).
@@ -89,33 +87,33 @@ Module NullPolicy <: Policy.
 
   Definition LocalT (l:loc) (ce : composite_env) (pct: control_tag) (ty : type) :
     PolicyResult (control_tag * val_tag * list loc_tag)%type :=
-    PolicySuccess (tt, tt, repeat tt (Z.to_nat (sizeof ce ty))).
+    Success (tt, tt, repeat tt (Z.to_nat (sizeof ce ty))).
   
   Definition DeallocT (l:loc) (ce : composite_env) (pct: control_tag) (ty : type) :
     PolicyResult (control_tag * val_tag * loc_tag) :=
-    PolicySuccess (tt, tt, tt).
+    Success (tt, tt, tt).
 
   Definition MallocT (l:loc) (pct: control_tag) (pt vt: val_tag) :
     PolicyResult (control_tag * val_tag * val_tag * val_tag * loc_tag) :=
-    PolicySuccess (tt, tt, tt, tt, tt).
+    Success (tt, tt, tt, tt, tt).
 
   Definition FreeT (l:loc) (pct: control_tag) (fpt pt vt: val_tag) :
     PolicyResult (control_tag * val_tag * val_tag * val_tag) :=
-    PolicySuccess (tt, tt, tt, tt).
+    Success (tt, tt, tt, tt).
 
   Definition ExtCallT (l:loc) (fn : string) (pct: control_tag) (args : list val_tag) :
-    PolicyResult (control_tag * val_tag) := PolicySuccess (tt,tt).
+    PolicyResult (control_tag * val_tag) := Success (tt,tt).
   
   Definition FieldT (l:loc) (ce: composite_env) (pct: control_tag) (vt: val_tag) (ty: type) (id: ident)
-    : PolicyResult val_tag := PolicySuccess tt.
+    : PolicyResult val_tag := Success tt.
 
   Definition PICastT (l:loc) (pct: control_tag) (pt: val_tag)  (lts : list loc_tag) (ty : type) :
-    PolicyResult val_tag := PolicySuccess tt.
+    PolicyResult val_tag := Success tt.
   Definition IPCastT (l:loc) (pct: control_tag) (vt: val_tag)  (lts : list loc_tag) (ty : type) :
-    PolicyResult val_tag := PolicySuccess tt.
+    PolicyResult val_tag := Success tt.
   Definition PPCastT (l:loc) (pct: control_tag) (vt: val_tag) (lts1 lts2 : list loc_tag) (ty : type) :
-    PolicyResult val_tag := PolicySuccess tt.
+    PolicyResult val_tag := Success tt.
   Definition IICastT (l:loc) (pct: control_tag) (vt: val_tag) (ty : type) : PolicyResult val_tag :=
-    PolicySuccess tt.
+    Success tt.
 
 End NullPolicy.
