policies/PVI.v
@@ -41,57 +41,59 @@ Module PVI <: Policy.
   Definition DefLT   : loc_tag := N.
   Definition InitT   : val_tag := N.
 
-  Definition print_tag (t : tag) : string :=
+  Definition print_vt (t : val_tag) : string :=
     match t with
-    | VT (Glob id) | LT (Glob id) => "Global " ++ (extern_atom id)
-    | VT (Dyn c) | LT (Dyn c) => "Dynamic"
-    | VT N | LT N => "N"
-    | CT c => "Next"
+    | Glob id => "Global " ++ (extern_atom id)
+    | Dyn c => "Dynamic"
+    | N => "N"
+    end.
+  Definition print_ct (t : control_tag) : string := "Next".
+  Definition print_lt (t : loc_tag) : string :=
+    match t with
+    | Glob id => "Global " ++ (extern_atom id)
+    | Dyn c => "Dynamic"
+    | N => "N"
     end.
 
+  Definition policy_state := unit.
+  Definition log (pstate:policy_state) (msg:string) := pstate.
+  Definition dump (pstate:policy_state) : string := "".
+  
   Definition color_eq (pt: val_tag) (lt: loc_tag) : bool :=
     match pt, lt with
     | Glob id1, Glob id2 => (id1 =? id2)%positive
     | Dyn c1, Dyn c2 => (c1 =? c2)%nat
     | _, _ => false
     end.
-  
-  (* Does not inherit from Policy, more like impersonates *)
-  Inductive PolicyResult (A: Type) :=
-  | PolicySuccess (res: A) 
-  | PolicyFail (r: string) (params: list tag).
-
-  Arguments PolicySuccess {_} _. 
-  Arguments PolicyFail {_} _ _.
-  
+    
   Definition inj_loc (s:string) (l:loc) : string :=
     s ++ " at " ++ (print_loc l).
   
   Definition LoadT (l:loc) (pct: control_tag) (pt vt: val_tag) (lts : list loc_tag) :
     PolicyResult val_tag :=
     match pt with
-    | N => PolicyFail (inj_loc "PVI || LoadT X Failure" l) ([CT pct;VT pt;VT vt]++(map LT lts))
-    | _ => if forallb (color_eq pt) lts then PolicySuccess vt 
-           else PolicyFail (inj_loc "PVI || LoadT tag_eq_dec Failure" l) ([CT pct;VT pt;VT vt]++(map LT lts))
+    | N => Fail (inj_loc "PVI || LoadT X Failure" l) PolicyFailure
+    | _ => if forallb (color_eq pt) lts then Success vt 
+           else Fail (inj_loc "PVI || LoadT tag_eq_dec Failure" l) PolicyFailure
     end.
 
   Definition StoreT (l:loc) (pct: control_tag) (pt vt: val_tag) (lts : list loc_tag) :
     PolicyResult (control_tag * val_tag * list loc_tag) :=
     match pt with
-    | N => PolicyFail (inj_loc "PVI || StoreT X Failure" l) ([CT pct;VT pt;VT vt]++(map LT lts))
-    | _ => if forallb (color_eq pt) lts then PolicySuccess (pct,vt,lts) 
-           else (PolicyFail (inj_loc "PVI || StoreT tag_eq_dec Failure" l) ([CT pct;VT pt;VT vt]++(map LT lts)))
+    | N => Fail (inj_loc "PVI || StoreT X Failure" l) PolicyFailure
+    | _ => if forallb (color_eq pt) lts then Success (pct,vt,lts) 
+           else Fail (inj_loc "PVI || StoreT tag_eq_dec Failure" l) PolicyFailure
     end.
   
   Definition BinopT (l:loc) (op : binary_operation) (pct: control_tag) (vt1 vt2 : val_tag) :
     PolicyResult (control_tag * val_tag) :=
     match vt1, vt2 with
-    | Dyn n, X =>  PolicySuccess (pct, vt1)
-    | Glob id, X => PolicySuccess (pct, vt1)
-    | _, _ => PolicySuccess (pct, vt2)
+    | Dyn n, X =>  Success (pct, vt1)
+    | Glob id, X => Success (pct, vt1)
+    | _, _ => Success (pct, vt2)
     end.
 
-  Definition ConstT (l:loc) (pct : control_tag) : PolicyResult val_tag := PolicySuccess N.
+  Definition ConstT (l:loc) (pct : control_tag) : PolicyResult val_tag := Success N.
 
   Definition GlobalT (ce : composite_env) (id : ident) (ty : type) : val_tag * val_tag * loc_tag :=
     (Glob id, N, Glob id).
@@ -101,36 +103,39 @@ Module PVI <: Policy.
   Definition LocalT (l:loc) (ce : composite_env) (pct : control_tag) (ty : type) :
     PolicyResult (control_tag * val_tag * (list loc_tag))%type :=
     let c := pct in
-    PolicySuccess (S c, Dyn c, repeat (Dyn c) (Z.to_nat (sizeof ce ty))).
+    Success (S c, Dyn c, repeat (Dyn c) (Z.to_nat (sizeof ce ty))).
   
   Definition DeallocT (l:loc) (ce : composite_env) (pct : control_tag) (ty : type) :
     PolicyResult (control_tag * val_tag * loc_tag) :=
-    PolicySuccess (pct, N, N).
+    Success (pct, N, N).
 
   Definition MallocT (l:loc) (pct: control_tag) (pt vt: val_tag) :
     PolicyResult (control_tag * val_tag * val_tag * val_tag * loc_tag) :=
     let c := pct in
-    PolicySuccess (S c, Dyn c, N, Dyn c, Dyn c).
+    Success (S c, Dyn c, N, Dyn c, Dyn c).
 
   Definition FreeT (l:loc) (pct: control_tag) (pt1 pt2 vt: val_tag) :
     PolicyResult (control_tag * val_tag * val_tag * val_tag) :=
-    PolicySuccess (pct, N, N, N).
+    Success (pct, N, N, N).
+
+  Definition ExtCallT (l:loc) (fn: string) (pct: control_tag) (args: list val_tag) :
+    PolicyResult (control_tag * val_tag) :=
+    Success (pct, N).
 
   (* Passthrough rules *)  
-  Definition CallT := (fun l pct fpt => PolicySuccess (Passthrough.CallT val_tag control_tag l pct fpt)).  
-  Definition ArgT := (fun l pct fpt vt idx ty => PolicySuccess (Passthrough.ArgT val_tag control_tag l pct fpt vt idx ty)).
-  Definition RetT := (fun l pct1 pct2 vt => PolicySuccess (Passthrough.RetT val_tag control_tag l pct1 pct2 vt)).
-  Definition AccessT := (fun l pct vt => PolicySuccess (Passthrough.AccessT val_tag control_tag l pct vt)).
-  Definition AssignT := (fun l pct vt1 vt2 => PolicySuccess (Passthrough.AssignT val_tag control_tag l pct vt1 vt2)).
-  Definition UnopT := (fun l op pct vt => PolicySuccess (Passthrough.UnopT val_tag control_tag l op pct vt)).
-  Definition SplitT := (fun l pct vt lbl => PolicySuccess (Passthrough.SplitT val_tag control_tag l pct vt lbl)).
-  Definition LabelT := (fun l pct lbl => PolicySuccess (Passthrough.LabelT control_tag l pct lbl)).
-  Definition ExprSplitT := (fun l pct vt => PolicySuccess (Passthrough.ExprSplitT val_tag control_tag l pct vt)).
-  Definition ExprJoinT := (fun l pct vt => PolicySuccess (Passthrough.ExprJoinT val_tag control_tag l pct vt)).
-  Definition ExtCallT := (fun l str pct fpt => PolicySuccess (Passthrough.ExtCallT val_tag control_tag InitT l str pct fpt)).
-  Definition FieldT := (fun l ce pct vt id ty => PolicySuccess (Passthrough.FieldT val_tag control_tag l ce pct vt id ty)).
-  Definition PICastT := (fun l pct pt lts ty => PolicySuccess (Passthrough.PICastT val_tag control_tag loc_tag l pct pt lts ty)).
-  Definition IPCastT := (fun l pct vt lts ty => PolicySuccess (Passthrough.IPCastT val_tag control_tag loc_tag l pct vt lts ty)).
-  Definition PPCastT := (fun l pct pt lts1 lts2 ty => PolicySuccess (Passthrough.PPCastT val_tag control_tag loc_tag l pct pt lts1 lts2 ty)).
-  Definition IICastT := (fun l pct vt ty => PolicySuccess (Passthrough.IICastT val_tag control_tag l pct vt ty)).
+  Definition CallT := Passthrough.CallT val_tag control_tag.  
+  Definition ArgT := Passthrough.ArgT val_tag control_tag.
+  Definition RetT := Passthrough.RetT val_tag control_tag.
+  Definition AccessT := Passthrough.AccessT val_tag control_tag.
+  Definition AssignT := Passthrough.AssignT val_tag control_tag.
+  Definition UnopT := Passthrough.UnopT val_tag control_tag.
+  Definition SplitT := Passthrough.SplitT val_tag control_tag.
+  Definition LabelT := Passthrough.LabelT control_tag.
+  Definition ExprSplitT := Passthrough.ExprSplitT val_tag control_tag.
+  Definition ExprJoinT := Passthrough.ExprJoinT val_tag control_tag.
+  Definition FieldT := Passthrough.FieldT val_tag control_tag.
+  Definition PICastT := Passthrough.PICastT val_tag control_tag loc_tag.
+  Definition IPCastT := Passthrough.IPCastT val_tag control_tag loc_tag.
+  Definition PPCastT := Passthrough.PPCastT val_tag control_tag loc_tag.
+  Definition IICastT := Passthrough.IICastT val_tag control_tag.
 End PVI.
